GeneralizedAlgebra/signatures/bipointed.lean
@@ -1,3 +1,19 @@
-import GeneralizedAlgebra.nouGAT
+import GeneralizedAlgebra.signatures.pointed
 
-def 𝔅 : GAT := ⦃ X : U, x : X, x' : X ⦄
+def 𝔅 : GAT := ⟨
+  ⦃ X : U, x : X, x' : X ⦄,
+
+  by
+    intro P
+    apply P.cons_D
+    apply P.EL_D
+    rw [WkTm]
+    have helper := P.VARSUCC_D [Ty.EL (Tm.VAR 0), Ty.UU] --[Ty.UU] (P.cons_D _ P.nil_D _ (P.UU_D _ _)) (Ty.EL (Tm.VAR 0)) (P.EL_D _ _ _ (P.VAR0_D _ _ _ _ _)) (Tm.VAR 0) Ty.UU (P.UU_D _ _)  -- (Ty.EL (Tm.VAR 1))
+    -- rw [WkTm] at helper
+    apply helper
+    have helper' := P.VAR0_D EMPTY P.nil_D Ty.UU (P.UU_D _ _)
+    rw [WkTy] at helper'
+    apply helper'
+
+
+  ⟩
