GeneralizedAlgebra/signatures/pointed.lean
@@ -1,4 +1,29 @@
 import GeneralizedAlgebra.nouGAT
 
-def 𝔓 : GAT := ⦃ X : U, x : X
-⦄
+
+def pointedLemma (P : indData) :
+  P.Tm_D
+    [Ty.UU]
+    (P.cons_D [] P.nil_D Ty.UU (P.UU_D [] P.nil_D))
+    (Ty.EL (Tm.VAR 0))
+    (P.EL_D [Ty.UU] (P.cons_D [] P.nil_D Ty.UU (P.UU_D [] P.nil_D)) (Tm.VAR 0) (P.VAR0_D [] P.nil_D Ty.UU (P.UU_D [] P.nil_D) (P.UU_D [Ty.UU] (P.cons_D [] P.nil_D Ty.UU (P.UU_D [] P.nil_D)))))
+    (Tm.VAR 0)
+  := by
+
+    have helper := P.VAR0_D EMPTY P.nil_D Ty.UU (P.UU_D _ _) (P.UU_D _ _)
+    -- rw [WkTy] at helper
+    sorry
+
+
+
+def 𝔓 : GAT := ⟨
+  ⦃ X : U, x : X ⦄,
+
+  by
+    intro P
+    apply P.cons_D
+    apply P.EL_D
+    have helper := P.VAR0_D EMPTY P.nil_D Ty.UU (P.UU_D _ _)
+    rw [WkTy] at helper
+    apply helper
+  ⟩
